code/streaming/Hacl.Streaming.Poly1305_128.fst
@@ -9,6 +9,8 @@ open Hacl.Streaming.Poly1305
 
 #set-options "--fuel 0 --ifuel 0 --z3rlimit 100"
 
+let k = poly1305_key
+
 /// Type abbreviation - makes KaRaMeL use pretty names in the generated code
 let poly1305_128_state = F.state_s (poly1305 M128) () (t M128) (k.I.s ())
 
